@@ -1,0 +1,10 @@
+/-
+`sys_close` meets its specification, given `argfd`, `myproc` and `fileclose`.
+-/
+import Xv6.ProofSysClose
+
+namespace Xv6
+
+theorem SysClose (AF : ARGFD) (MP : MYPROC) (FC : FILECLOSE) : SYSCLOSE := sys_close_proof AF MP FC
+
+end Xv6
